working on equiv

software-foundations/A015equiv.v
@@ -1,1 +1,163 @@
 Require Export A014imp.
+
+
+Definition aequiv (a1 a2 : aexp) : Prop :=
+  forall (st:state),
+    aeval st a1 = aeval st a2.
+
+Definition bequiv (b1 b2 : bexp) : Prop :=
+  forall (st:state),
+    beval st b1 = beval st b2.
+
+Definition cequiv (c1 c2 : com) : Prop :=
+  forall (st st' : state),
+    (c1 / st || st') <-> (c2 / st || st').
+
+
+
+(* Exercise: 2 stars (equiv_classes) *)
+
+Definition prog_a : com :=
+  WHILE BNot (BLe (AId X) (ANum 0)) DO
+    X ::= APlus (AId X) (ANum 1)
+  END.
+
+Definition prog_b : com :=
+  IFB BEq (AId X) (ANum 0) THEN
+    X ::= APlus (AId X) (ANum 1);;
+    Y ::= ANum 1
+  ELSE
+    Y ::= ANum 0
+  FI;;
+  X ::= AMinus (AId X) (AId Y);;
+  Y ::= ANum 0.
+
+Definition prog_c : com :=
+  SKIP.
+
+Definition prog_d : com :=
+  WHILE BNot (BEq (AId X) (ANum 0)) DO
+    X ::= APlus (AMult (AId X) (AId Y)) (ANum 1)
+  END.
+
+Definition prog_e : com :=
+  Y ::= ANum 0.
+
+Definition prog_f : com :=
+  Y ::= APlus (AId X) (ANum 1);;
+  WHILE BNot (BEq (AId X) (AId Y)) DO
+    Y ::= APlus (AId X) (ANum 1)
+  END.
+
+Definition prog_g : com :=
+  WHILE BTrue DO
+    SKIP
+  END.
+
+Definition prog_h : com :=
+  WHILE BNot (BEq (AId X) (AId X)) DO
+    X ::= APlus (AId X) (ANum 1)
+  END.
+
+Definition prog_i : com :=
+  WHILE BNot (BEq (AId X) (AId Y)) DO
+    X ::= APlus (AId Y) (ANum 1)
+  END.
+
+
+
+Definition equiv_classes : list (list com) :=
+  [[prog_a ; prog_g ] ;
+    [prog_c ; prog_h] ;
+    [prog_i] ;
+    [prog_f] ;
+    [prog_e] ;
+    [prog_b]
+  ].
+(* GRADE_TEST 2: check_equiv_classes equiv_classes *)
+
+
+Theorem aequiv_example:
+  aequiv (AMinus (AId X) (AId X)) (ANum 0).
+Proof.
+  unfold aequiv. intros.
+  unfold aeval.
+  assert (forall n : nat, n - n = 0).
+  intros. induction n. reflexivity. assumption.
+  apply H.
+Qed.
+
+Theorem bequiv_example:
+  bequiv (BEq (AMinus (AId X) (AId X)) (ANum 0)) BTrue.
+Proof.
+  unfold bequiv. intros. unfold beval. simpl. rewrite minus_diag. reflexivity.
+Qed.
+
+Theorem skip_left: forall c,
+  cequiv
+     (SKIP;; c)
+     c.
+Proof.
+  unfold cequiv. intros.
+  split; intros.
+
+  Case "→".
+  inversion H; subst.
+  inversion H2; subst.
+  assumption.
+
+  Case "←".
+  apply E_Seq with (st' := st).
+  apply E_Skip. assumption.
+Qed.
+
+
+(* Exercise: 2 stars (skip_right) *)
+
+Theorem skip_right: forall c,
+  cequiv
+    (c;; SKIP)
+    c.
+Proof.
+  unfold cequiv. intros.
+  split; intros.
+
+  inversion H; subst. inversion H5; subst. assumption.
+  apply E_Seq with (st' := st'). assumption. apply E_Skip.
+Qed.
+
+
+Theorem IFB_true_simple: forall c1 c2,
+  cequiv
+    (IFB BTrue THEN c1 ELSE c2 FI)
+    c1.
+Proof.
+  unfold cequiv. intros.
+  split; intros.
+
+  Case "->".
+  inversion H; subst. assumption. inversion H5.
+
+  Case "<-".
+  apply E_IfTrue. reflexivity. assumption.
+Qed.
+
+(* Exercise: 2 stars (IFB_false) *)
+Theorem IFB_false: forall b c1 c2,
+  bequiv b BFalse ->
+  cequiv
+    (IFB b THEN c1 ELSE c2 FI)
+    c2.
+Proof.
+  unfold bequiv. unfold cequiv. intros.
+  split; intros.
+
+  inversion H0; subst; try assumption.
+  specialize H with st.
+  inversion H.
+  rewrite H2 in H6. inversion H6.
+
+  specialize H with st.
+  inversion H.
+  apply E_IfFalse; try assumption.
+Qed.
